Opriginal version of Computation, Step and Fail are derived

src/Lambda.v
@@ -1,17 +1,14 @@
-Require Import Monads.Tactics.
-Require Import Monads.Utils.
-
 From Coq Require Import List Lia Arith.
 
-CoInductive Computation (A:Type) : Type :=
+CoInductive Computation (A: Type) : Type :=
 | Return : A -> Computation A
-| Bind : forall (B:Type), Computation B-> (B-> Computation A)-> Computation A
-| Fail
-| Step : Computation A -> Computation A.
+| Bind : forall (B:Type), Computation B-> (B-> Computation A)-> Computation A.
+
 Arguments Return {A}.
 Arguments Bind {A B}.
-Arguments Step {A}.
-Arguments Fail {A}.
+
+Definition Fail {A} := Return (@None A).
+Definition Step {A} (x: Computation A):= (Bind (Return tt) (fun (y: unit) => x)).
 
 Axiom Bind_On_Return: forall (A B: Type) (x: A) (f: A -> Computation B), 
 Bind (Return x) f = f x.
@@ -26,32 +23,10 @@ Notation "var <- c ; rest" :=
 Definition frob {A}(x: Computation A) :=
 match x with 
 | Return y => Return y
-| Bind y f => Bind y f
-| Fail     => Fail
-| Step t   => Step t end.
+| Bind y f => Bind y f end.
 
 Lemma frob_eq {A}: forall (x: Computation A), x = frob x.
 Proof. destruct x; reflexivity. Qed.
-
-CoInductive bisim {A} : Computation A -> Computation A -> Prop :=
-| BisimRtrn   : forall x, bisim (Return x) (Return x)
-| BisimBind  : forall (B: Type) (f: B -> Computation A) x, bisim (Bind x f) (Bind x f)
-| BisimStep : forall x y, bisim x y -> bisim (Step x) (Step y)
-| BisimStepL : forall x y, bisim x y -> bisim (Step x) y
-| BisimStepR : forall x y, bisim x y -> bisim  x (Step y)
-| BisimFail: bisim Fail Fail.
-
-Theorem bisim_refl {A}: forall (a: Computation A), bisim a a.
-Proof. cofix CIH.  intros. destruct a; constructor; constructor; apply CIH. Qed.
-
-Theorem bisim_symm {A}: forall (a b: Computation A), bisim a b -> bisim b a.
-Proof. cofix CIH. intros. inversion H; subst; constructor.
--  inversion H; 
-repeat (apply CIH in H0; assumption;
-  apply CIH in H0; assumption).
-- apply CIH in H0; assumption.
-- apply CIH in H0; assumption. Qed.
-
 
 Definition const :=nat. 
 
@@ -66,72 +41,67 @@ Inductive value: Type :=
   | Clos: term -> list value -> value.
 
 Definition env := list value.
+Definition CompFail (A: Type) := Computation (option A).
 
-CoFixpoint bs (t: term) (e:env): (Computation value) :=
+CoFixpoint bs (t: term) (e:env): (CompFail value) :=
 match t with 
- | Const i => Return (Int i)
+ | Const i => Return (Some (Int i))
  | Var n   => match (nth_error e n) with 
-           | Some v => Return v
+           | Some v => Return (Some v)
            | None   => Fail end
- | Fun a => Return (Clos a e) 
+ | Fun a => Return (Some (Clos a e))
  | App a b => v1 <- bs a e ; v2 <- bs b e ; match v1 with 
-                                    | Int n    => Fail 
-                                    | Clos x y => Step (bs x (v2::y))
+                                    | None     => Fail
+                                    | Some (Int n)    => Fail 
+                                    | Some (Clos x y) => match v2 with 
+                                                          | None => Fail 
+                                                          | Some t => Step (bs x (t::y)) end
                                                    end end.
 
 CoFixpoint never := @Step value never.
 
-Lemma bisim_successful: forall e, bisim ( bs (Const 2) e) (Return (Int 2)).
-Proof. intros. rewrite frob_eq with (x:=bs (Const 2) e). simpl. constructor. Qed.
-
-Lemma bisim_fail: forall e, bisim (bs (App (Const 1) (Const 2)) e) Fail.
-Proof. intros. rewrite frob_eq with (x:=bs (App (Const 1) (Const 2)) e). simpl. 
-rewrite frob_eq with (x:=bs (Const 1) e). rewrite frob_eq with (x:=bs (Const 2) e).
-simpl. rewrite Bind_On_Return. rewrite Bind_On_Return. constructor. Qed.
-
-Definition delta := Fun (App (Var 0) (Var 0)).
-Definition omega := App delta delta.
-
-Lemma bisim_infinite: forall e, bisim (bs omega e) never.
-Proof.  intros. rewrite frob_eq with (x:=bs omega e).  simpl. 
-rewrite frob_eq with (x:=bs delta e). simpl. rewrite Bind_On_Return. 
-rewrite Bind_On_Return. constructor. cofix CIH. 
- rewrite frob_eq with (x:=(bs (App (Var 0) (Var 0)) (Clos (App (Var 0) (Var 0)) e :: e))). simpl. 
- rewrite frob_eq with (x:=bs (Var 0) (Clos (App (Var 0) (Var 0)) e :: e)). simpl. rewrite Bind_On_Return. 
-rewrite Bind_On_Return. constructor. apply CIH. Qed.
-
 Inductive val {A}: Computation A -> A -> Prop :=
- value_return : forall a:A, val (Return a) a
-| value_step : forall (x:Computation A)(a:A), val x a -> val (Step x) a.
+| value_return : forall a:A, val (Return a) a
+| value_bind : forall (a: A) (B: Type) (b: B) (c: Computation B)
+         (f: B -> Computation A), val c b -> val (f b) a -> val (Bind c f) a.
+
+Lemma value_step {A}: forall (x:Computation A)(a:A), val x a -> val (Step x) a.
+Proof. intros. induction H. 
+- unfold Step. rewrite Bind_On_Return. constructor.
+- unfold Step. rewrite Bind_On_Return. apply value_bind with (b:=b); assumption. Qed.
 
 
 CoInductive Eqp {A}: Computation A -> Computation A -> Prop :=
- eqp_value : forall (x y:Computation A)(a:A), val x a -> val y a -> (Eqp x y)
+| eqp_value : forall (x y:Computation A)(a:A), val x a -> val y a -> (Eqp x y)
 | eqp_step : forall (x y:Computation A), Eqp x y -> Eqp (Step x) (Step y)
-| eqp_fail: Eqp Fail Fail.
+| eqp_equal: forall (x :Computation A), Eqp x x.
 
 
-Theorem eqp_refl_return {A}: forall (x: A), Eqp (Return x) (Return x).
-Proof.  intros. apply eqp_value with (a:=x).  constructor. constructor. Qed.
+Definition ret {A} (x:A) := Return (Some x).
 
-Lemma eqp_successful: forall e, Eqp ( bs (Const 2) e) (Return (Int 2)).
-Proof. intros. rewrite frob_eq with (x:=bs (Const 2) e). simpl. apply eqp_refl_return. Qed.
+Lemma eqp_successful: forall e, Eqp ( bs (Const 2) e) (ret (Int 2)).
+Proof. intros. rewrite frob_eq with (x:=bs (Const 2) e). simpl. constructor. Qed.
 
 Lemma eqp_failure: forall e, Eqp (bs (App (Const 1) (Const 2)) e) Fail.
 Proof. intros. rewrite frob_eq with (x:=bs (App (Const 1) (Const 2)) e). simpl.
 rewrite frob_eq with (x:=bs (Const 1) e).
 rewrite frob_eq with (x:=bs (Const 2) e). simpl. rewrite Bind_On_Return. rewrite Bind_On_Return. constructor. Qed.
 
-Lemma eqp_never:  Eqp (Step never) never.
-Proof. cofix CIH. rewrite frob_eq with (x:=never). simpl. constructor. assumption. Qed.
+CoFixpoint Never := @Step (option value) Never.
 
-Lemma eqp_infinite: forall e, Eqp (bs omega e) never.
+Lemma eqp_never:  Eqp (Step Never) Never.
+Proof. cofix CIH. rewrite frob_eq with (x:=Never). simpl. constructor. assumption. Qed.
+
+Definition delta := Fun (App (Var 0) (Var 0)).
+Definition omega := App delta delta.
+
+Lemma eqp_infinite: forall e, Eqp (bs omega e) Never.
 Proof.  intros. rewrite frob_eq with (x:=bs omega e).  simpl. 
 rewrite frob_eq with (x:=bs delta e). simpl. rewrite Bind_On_Return. 
-rewrite Bind_On_Return. rewrite frob_eq with (x:=never). simpl. constructor. cofix CIH. 
- rewrite frob_eq with (x:=(bs (App (Var 0) (Var 0)) (Clos (App (Var 0) (Var 0)) e :: e))). simpl. 
- rewrite frob_eq with (x:=bs (Var 0) (Clos (App (Var 0) (Var 0)) e :: e)). simpl. rewrite Bind_On_Return. 
-rewrite Bind_On_Return.  rewrite frob_eq with (x:=never). simpl. constructor. apply CIH. Qed.
+rewrite Bind_On_Return. rewrite frob_eq with (x:=Never). simpl. constructor. cofix CIH. 
+rewrite frob_eq with (x:=(bs (App (Var 0) (Var 0)) (Clos (App (Var 0) (Var 0)) e :: e))). simpl. 
+rewrite frob_eq with (x:=bs (Var 0) (Clos (App (Var 0) (Var 0)) e :: e)). simpl. rewrite Bind_On_Return. 
+rewrite Bind_On_Return.  rewrite frob_eq with (x:=Never). simpl. constructor. apply CIH. Qed.
 
 
 
